theories/examples/buffers.v
@@ -3,24 +3,17 @@ From iris.proofmode Require Export tactics.
 From iris.prelude Require Import options.
 From melocoton Require Import named_props.
 From melocoton.interop Require Import basics basics_resources.
-From melocoton.lang_to_mlang Require Import lang weakestpre.
-From melocoton.interop Require Import lang weakestpre update_laws wp_utils wp_ext_call_laws wp_simulation.
+From melocoton.interop Require Import lang weakestpre update_laws wp_utils prims_proto.
+From melocoton.language Require Import weakestpre progenv.
 From melocoton.c_interop Require Import rules notation.
 From melocoton.ml_lang Require Import notation lang_instantiation.
 From melocoton.c_lang Require Import mlang_instantiation lang_instantiation.
-From melocoton.ml_lang Require proofmode.
-From melocoton.c_lang Require notation proofmode.
-From melocoton.mlanguage Require Import progenv.
-From melocoton.mlanguage Require weakestpre.
-From melocoton.linking Require Import lang weakestpre.
+From melocoton.ml_lang Require primitive_laws proofmode.
+From melocoton.c_lang Require Import notation proofmode.
 From melocoton.examples Require Import compression.
 
 
-Section C_prog.
-Import melocoton.c_lang.notation melocoton.c_lang.proofmode.
-
-Context `{SI:indexT}.
-Context `{!heapG_C Σ, !heapG_ML Σ, !invG Σ, !primitive_laws.heapG_ML Σ, !wrapperG Σ}.
+Section C_code.
 
 (** our code differs from the original in the paper as follows:
 
@@ -56,18 +49,16 @@ Definition buf_alloc_code (cap : expr) : expr :=
   CAMLlocal: "bk" in 
   CAMLlocal: "bf" in 
   CAMLlocal: "bf2" in 
-  let: "bfref" := malloc (#1) in
   "bk" <- caml_alloc_custom ( ) ;;
-  Custom_contents ( *"bk" ) :=  Val_int (cap) ;;
+  (Custom_contents ( *"bk" ) :=  malloc(Int_val (cap))) ;;
   "bf"    <- caml_alloc (#2, #0) ;;
   "bf2"   <- caml_alloc (#2, #0) ;;
-  "bfref" <- caml_alloc (#1, #0) ;;
-  Store_field ( &Field( *"bfref", #0), Val_int (#0)) ;;
-  Store_field ( &Field( *"bf", #0), *"bfref") ;;
+  let: "bfref" := caml_alloc (#1, #0) in
+  Store_field ( &Field(  "bfref", #0), Val_int (#0)) ;;
+  Store_field ( &Field( *"bf", #0), "bfref") ;;
   Store_field ( &Field( *"bf", #1), *"bf2") ;;
   Store_field ( &Field( *"bf2", #0), cap) ;;
   Store_field ( &Field( *"bf2", #1), *"bk") ;;
-  free ("bfref", #1) ;;
   CAMLreturn: * "bf" unregistering ["bk", "bf", "bf2"].
 Definition buf_alloc_fun := Fun [BNamed "cap"] (buf_alloc_code "cap") .
 Definition buf_alloc_name := "buf_alloc".
@@ -109,5 +100,213 @@ Definition wrap_compress_code (bf1 bf2 : expr) : expr :=
 Definition wrap_compress_fun := Fun [BNamed "bf1"; BNamed "bf2"] (wrap_compress_code "bf1" "bf2").
 Definition wrap_compress_name := "wrap_compress".
 
-End C_prog.
+Definition buf_lib_prog : lang_prog C_lang :=
+  <[wrap_compress_name := wrap_compress_fun]> (
+  <[wrap_max_len_name  := wrap_max_len_fun]> (
+  <[buf_upd_name       := buf_upd_fun]> (
+  <[buf_alloc_name     := buf_alloc_fun]>
+    buffy_env ))).
 
+End C_code.
+
+Section Specs.
+
+  Context `{SI:indexT}.
+  Context `{!heapG_C Σ, !heapG_ML Σ, !invG Σ, !primitive_laws.heapG_ML Σ, !wrapperG Σ}.
+
+  Definition wrap_funcs_code E e Ψ : prog_environ C_lang Σ := {|
+    penv_prog  := buf_lib_prog ;
+    penv_proto := prims_proto E e Ψ |}.
+
+  Definition isBufferForeignBlock (γ : lloc) (b:buffer) cap fid : iProp Σ := 
+      ∃ (ℓbuf : loc) vused vrest, 
+        "Hγfgnpto" ∷ γ ↦foreign (#ℓbuf)
+      ∗ "#Hγfgnsim" ∷ γ ~foreign~ fid
+      ∗ "Hℓbuf" ∷ ℓbuf ↦C∗ (vused++vrest)
+      ∗ "%HisBuf" ∷ ⌜isBuffer vused b⌝
+      ∗ "<-" ∷ ⌜length (vused++vrest) = cap⌝.
+
+  Definition isBufferRecord (lv : lval) (b:buffer) (cap:nat) : iProp Σ :=
+    ∃ (γ γref γaux γfgn : lloc) (used : nat) fid,
+        "->" ∷ ⌜lv = Lloc γ⌝
+      ∗ "#Hγbuf" ∷ γ ↦imm (TagDefault, [Lloc γref; Lloc γaux])
+      ∗ "Hγusedref" ∷ γref ↦mut (TagDefault, [Lint used])
+      ∗ "#Hγaux" ∷ γaux ↦imm (TagDefault, [Lint cap; Lloc γfgn])
+      ∗ "Hbuf" ∷ isBufferForeignBlock γfgn b cap fid
+      ∗ "->" ∷ ⌜used = length b⌝.
+
+  Definition isBufferRecordML (v : MLval) (b:buffer) (cap:nat) : iProp Σ :=
+    ∃ (ℓML:loc) (used fid:nat) γfgn, 
+      "->" ∷ ⌜v = (ML_lang.LitV ℓML, (ML_lang.LitV cap, ML_lang.LitV (LitForeign fid)))%MLV⌝ 
+    ∗ "HℓbufML" ∷ ℓML ↦M ML_lang.LitV used
+    ∗ "Hbuf" ∷ isBufferForeignBlock γfgn b cap fid
+    ∗ "->" ∷ ⌜used = length b⌝.
+
+  Lemma bufToML lv b c θ:
+      GC θ
+   -∗ isBufferRecord lv b c
+  ==∗ GC θ ∗ ∃ v, isBufferRecordML v b c ∗ lv ~~ v.
+  Proof.
+    iIntros "HGC H". iNamed "H". iNamed "Hbuf".
+    iMod (mut_to_ml _ ([ML_lang.LitV (length b)]) with "[$HGC $Hγusedref]") as "(HGC&(%ℓML&HℓbufML&#HγML))".
+    1: by cbn.
+    iModIntro. iFrame "HGC".
+    iExists _. iSplitL.
+    { iExists ℓML, _, fid, γfgn. unfold named.
+      iSplit; first done. iFrame "HℓbufML". iSplit; last done.
+      iExists ℓbuf, vused, vrest.
+      unfold named. by iFrame "Hγfgnpto Hℓbuf Hγfgnsim". }
+    { cbn. iExists _, _, _. iSplitL; first done.
+      iFrame "Hγbuf".
+      iSplitL; first (iExists _; iSplit; done).
+      iExists _, _, _. iSplit; first done.
+      iFrame "Hγaux". iSplit; first done.
+      iExists _; iSplit; done. }
+  Qed.
+
+  Lemma bufToC v b c lv θ:
+      GC θ
+   -∗ isBufferRecordML v b c
+   -∗ lv ~~ v
+  ==∗ GC θ ∗ isBufferRecord lv b c.
+  Proof.
+    iIntros "HGC H Hsim". iNamed "H". iNamed "Hbuf".
+    iDestruct "Hsim" as "#(%γ&%&%&->&Hγbuf&(%γref&->&Hsim)&%γaux&%&%&->&Hγaux&->&%γfgn2&->&Hγfgnsim2)".
+    iPoseProof (lloc_own_foreign_inj with "Hγfgnsim2 Hγfgnsim [$]") as "(HGC&%Hiff)".
+    destruct Hiff as [_ ->]; last done.
+    iMod (ml_to_mut with "[$HGC $HℓbufML]") as "(HGC&(%ℓvs&%γref2&Hγusedref&#Hsim2&#Hγrefsim))".
+    iPoseProof (lloc_own_pub_inj with "Hsim2 Hsim [$]") as "(HGC&%Hiff)".
+    destruct Hiff as [_ ->]; last done.
+    iModIntro. iFrame "HGC".
+    iExists _, _, _, _, _, _. unfold named.
+    iSplit; first done.
+    iFrame "Hγbuf". iFrame "Hγaux".
+    iSplitL "Hγusedref".
+    { destruct ℓvs as [|ℓvs [|??]]; cbn; try done.
+      all: iDestruct "Hγrefsim" as "[-> ?]"; try done. }
+    { iSplit; last done.
+      cbn. iExists _, _, _. unfold named. iFrame "Hγfgnpto Hγfgnsim Hℓbuf".
+      iPureIntro; done. }
+  Qed.
+
+
+  Import melocoton.ml_lang.notation.
+
+  Definition buf_alloc_spec_ML s vv Φ : iProp Σ :=
+    ∃ (z:Z),
+      ⌜(0 < z)%Z⌝
+    ∗ ⌜s = buf_alloc_name⌝
+    ∗ ⌜vv = [ #z ]⌝
+    ∗ ▷ (∀ v, isBufferRecordML v [] (Z.to_nat z) -∗ Φ v).
+
+End Specs.
+
+Section Proofs.
+
+  Context `{SI:indexT}.
+  Context `{!heapG_C Σ, !heapG_ML Σ, !invG Σ, !primitive_laws.heapG_ML Σ, !wrapperG Σ}.
+
+  Lemma buf_alloc_correct E1 E2 e Ψ :
+    wrap_proto buf_alloc_spec_ML ⊑ prog_proto E2 buf_lib_prog (prims_proto E1 e Ψ).
+  Proof.
+    iIntros (s ws Φ) "H". iNamed "H".
+    iDestruct "Hproto" as "(%cap&%Hcap&->&->&HΦ')".
+    cbn. unfold prog_proto. solve_lookup_fixed.
+    destruct lvs as [|lv [|??]]; first done.
+    all: cbn; iDestruct "Hsim" as "(->&H)"; try done.
+    destruct ws as [|w [|??]]; try (eapply Forall2_length in Hrepr; cbn in Hrepr; done).
+    eapply Forall2_cons_inv_l in Hrepr as (wcap&?&Hlval&_&?); simplify_eq.
+    cbn. iExists _. solve_lookup_fixed.
+    iSplit; first done. iNext.
+    wp_apply (wp_CAMLlocal with "HGC"); [done..|].
+    iIntros (ℓbk) "(HGC&Hℓbk)"; wp_pures.
+    wp_apply (wp_CAMLlocal with "HGC"); [done..|].
+    iIntros (ℓbf) "(HGC&Hℓbf)"; wp_pures.
+    wp_apply (wp_CAMLlocal with "HGC"); [done..|].
+    iIntros (ℓbf2) "(HGC&Hℓbf2)". wp_finish.
+    wp_apply (wp_alloc_foreign with "HGC"); [done..|].
+    iIntros (θ1 γbk wbk) "(HGC&Hγbk&%Hbk'1)".
+    wp_apply (store_to_root with "[$HGC $Hℓbk]"); [done..|].
+    iIntros "(HGC&Hℓbk)". wp_pures.
+    wp_apply (load_from_root with "[$HGC $Hℓbk]"); [done..|].
+    iIntros (w) "(Hℓbk&HGC&%Hbk'1b)".
+    wp_apply (wp_val2int with "HGC"); [try done..|].
+    1: by eapply repr_lval_lint.
+    iIntros "HGC".
+    wp_apply (wp_Malloc); [try done..|].
+    iIntros (ℓbts) "(Hbts&_)".
+    wp_apply (wp_write_foreign with "[$HGC $Hγbk]"); [try done..|].
+    iIntros "(HGC&Hγbk)". wp_pure _.
+    wp_apply (wp_alloc TagDefault with "HGC"); [done..|].
+    iIntros (θ2 γbf wbf) "(HGC&Hγbf&%Hbf'1)".
+    wp_apply (store_to_root with "[$HGC $Hℓbf]"); [done..|].
+    iIntros "(HGC&Hℓbf)". wp_pure _.
+    wp_apply (wp_alloc TagDefault with "HGC"); [done..|].
+    iIntros (θ3 γbf2 wbf2) "(HGC&Hγbf2&%Hbf2'1)".
+    wp_apply (store_to_root with "[$HGC $Hℓbf2]"); [done..|].
+    iIntros "(HGC&Hℓbf2)". wp_pure _.
+    wp_apply (wp_alloc TagDefault with "HGC"); [done..|].
+    iIntros (θ4 γbfref wbfref) "(HGC&Hγbfref&%Hbfref'1)".
+    wp_pure _.
+    wp_apply (wp_int2val with "HGC"); [done..|].
+    iIntros (wunit) "(HGC&%Hwunit)".
+    wp_apply (wp_modify with "[$HGC $Hγbfref]"); [done..|].
+    iIntros "(HGC&Hγbfref)".
+    wp_pure _.
+    wp_apply (load_from_root with "[$HGC $Hℓbf]"); [done..|].
+    iIntros (wbf'4) "(Hℓbf&HGC&%Hbf'4)".
+    wp_apply (wp_modify with "[$HGC $Hγbf]"); [done..|].
+    iIntros "(HGC&Hγbf)".
+    wp_pure _.
+    wp_apply (load_from_root with "[$HGC $Hℓbf]"); [done..|].
+    iIntros (wbf'4') "(Hℓbf&HGC&%Hbf'4')".
+    wp_apply (load_from_root with "[$HGC $Hℓbf2]"); [done..|].
+    iIntros (wbf2'4) "(Hℓbf2&HGC&%Hbf2'4)".
+    wp_apply (wp_modify with "[$HGC $Hγbf]"); [done..|].
+    iIntros "(HGC&Hγbf)".
+    wp_pure _.
+    wp_apply (load_from_root with "[$HGC $Hℓbf2]"); [done..|].
+    iIntros (wbf2'4') "(Hℓbf2&HGC&%Hbf2'4')".
+    wp_apply (wp_modify with "[$HGC $Hγbf2]"); [try done..|].
+    1: by eapply repr_lval_lint.
+    iIntros "(HGC&Hγbf2)".
+    wp_pure _.
+
+    wp_apply (load_from_root with "[$HGC $Hℓbf2]"); [done..|].
+    iIntros (wbf2'4'') "(Hℓbf2&HGC&%Hbf2'4'')".
+    wp_apply (load_from_root with "[$HGC $Hℓbk]"); [done..|].
+    iIntros (wbk'4') "(Hℓbk&HGC&%Hbk'4')".
+    wp_apply (wp_modify with "[$HGC $Hγbf2]"); [done..|].
+    iIntros "(HGC&Hγbf2)".
+    wp_pure _.
+
+    wp_apply (load_from_root with "[$HGC $Hℓbf]"); [done..|].
+    iIntros (wbf'4'') "(Hℓbf&HGC&%Hbf'4'')". wp_pure _.
+    wp_apply (wp_CAMLunregister1 with "[$HGC $Hℓbk]"); [done..|].
+    iIntros "HGC". wp_pure _.
+    wp_apply (wp_CAMLunregister1 with "[$HGC $Hℓbf]"); [done..|].
+    iIntros "HGC". wp_pure _.
+    wp_apply (wp_CAMLunregister1 with "[$HGC $Hℓbf2]"); [done..|].
+    iIntros "HGC". wp_pure _.
+    change (Z.to_nat 0) with 0.
+    change (Z.to_nat 1) with 1.
+    change (Z.to_nat 2) with 2.
+    cbn.
+    iMod (freeze_to_immut with "[$HGC $Hγbf]") as "(HGC&Hγbf)".
+    iMod (freeze_to_immut with "[$HGC $Hγbf2]") as "(HGC&Hγbf2)".
+    iMod (freeze_to_mut with "[$HGC $Hγbfref]") as "(HGC&Hγbfref)".
+    iAssert (isBufferRecord (Lloc γbf) [] (Z.to_nat cap)) with "[Hγbk Hγbf Hγbf2 Hγbfref Hbts]" as "Hbuffer".
+    { iDestruct "Hγbk" as "(Hγbk'&%fid&#Hfid)".
+      assert (∃ k, Z.of_nat k = cap) as (ncap&<-) by (exists (Z.to_nat cap); lia).
+      rewrite !Nat2Z.id.
+      iExists γbf, γbfref, γbf2, γbk, 0, fid. unfold named. iFrame.
+      iSplit; first done. iSplit; last done.
+      iExists ℓbts, [], (replicate ncap None). unfold named, lstore_own_foreign.
+      iFrame. iFrame "Hfid". iSplitL; first by iExists fid. iPureIntro; split_and!.
+      1: done.
+      cbn. by rewrite replicate_length. }
+    iMod (bufToML with "HGC Hbuffer") as "(HGC&%vv&Hbuffer&#Hsim)".
+    iModIntro. iApply ("Cont" with "HGC (HΦ' Hbuffer) Hsim [//]").
+  Qed.
+
+End Proofs.
