theories/c_lang/proofmode.v
@@ -15,13 +15,13 @@ Proof. by intros ->. Qed.
 Ltac solve_lookup_fixed := let rec go := match goal with
   [ |- context[ @lookup _ _ (@gmap _ ?eqdec _ _) _ ?needle (insert ?key ?val ?rem)]] =>
     (unify key needle; rewrite (@lookup_insert _ _ _ _ _ _ _ _ _ _ _ _ rem key val)) ||
-    (rewrite (@lookup_insert_ne _ _ _ _ _ _ _ _ _ _ _ _ rem key needle val); [go|congruence])
+    (rewrite (@lookup_insert_ne _ _ _ _ _ _ _ _ _ _ _ _ rem key needle val); [go|first [congruence|done]])
 | [ |- context[ @lookup _ _ (@gmap _ ?eqdec _ _) _ ?needle (delete ?key ?rem)]] => 
       (unify key needle; rewrite (@lookup_delete _ _ _ _ _ _ _ _ _ _ _ _ rem key)) ||
-      (rewrite (@lookup_delete_ne _ _ _ _ _ _ _ _ _ _ _ _ rem key needle); [go|congruence])
+      (rewrite (@lookup_delete_ne _ _ _ _ _ _ _ _ _ _ _ _ rem key needle); [go|first [congruence|done]])
 | [ |- context[ @lookup _ _ (@gmap _ ?eqdec _ _) _ ?needle (singletonM ?key ?val)]] =>
     (unify key needle; rewrite (@lookup_singleton _ _ _ _ _ _ _ _ _ _ _ _ key val)) ||
-    (rewrite (@lookup_singleton_ne _ _ _ _ _ _ _ _ _ _ _ _ key needle val); congruence)
+    (rewrite (@lookup_singleton_ne _ _ _ _ _ _ _ _ _ _ _ _ key needle val); first [congruence|done])
 | [ |- context[ @lookup _ _ (@gmap _ ?eqdec _ _) _ ?needle ∅]] => 
     rewrite (@lookup_empty _ _  _ _ _ _ _ _ _ _ _ _ needle) end in repeat (progress (unfold subst; try go; simpl)).
 
